completed week 7 mini assignment

300 ANU Computing/Theoretical Computer Science/dafny/week7_tutorial.dfy
@@ -48,7 +48,7 @@ function lookup (target: int, tree: Tree) : bool {
 
 
 // Binary Search Tree
-ghost predicate is_bst (tree: Tree) {
+ghost predicate is_binary_search_tree (tree: Tree) {
     match tree {
         case Emp => true
         case Node (left_node, i_main_node, right_node) => 
@@ -58,7 +58,7 @@ ghost predicate is_bst (tree: Tree) {
             target < i_main_node) &&
         (forall target: int :: is_in (target, right_node) ==> 
             target > i_main_node) && 
-        is_bst(left_node) && is_bst(right_node)
+        is_binary_search_tree(left_node) && is_binary_search_tree(right_node)
     }
 }
 // Returns either true or false.
@@ -96,29 +96,57 @@ ghost predicate is_bst (tree: Tree) {
 // Now consider the function insert and the lemma insert bst.
 
 
-lemma {:induction false} is_in_lookup(tree: Tree, target: int)
-    requires is_bst(tree)
-    ensures (is_in(target, tree)) == (is_in(target, tree)){
-        // match tree{
-        //     case Emp => 
-        //     case Node (left_node, i_main_node, right_node) =>  
-        // }
+lemma is_in_lookup(tree: Tree, target: int)
+    requires is_binary_search_tree(tree)
+    ensures (is_in(target, tree)) == (lookup(target, tree)){
     }
 
-
-
-// Given functions
-function insert (j: int, t: Tree): Tree {
-    match t { case Emp => Node (Emp, j, Emp)
-        case Node (l, i, r) =>
-        if (j < i) then Node (insert (j, l), i, r)
-        else if (j > i) then Node (l, i, insert (j, r)) else t
-    }
-}
 
 lemma insert_bst (j: int, t: Tree)
-requires is_bst (t)
-ensures is_bst (insert (j, t))
+requires is_binary_search_tree (t)
+ensures lookup(j, t) == is_in(j, t){
+
+}
+/* Proof by hand:
+We show that all t: T that are binary search trees satisfy
+lookup(j, t) == is_in(j, t) for all j: int.
+
+More formally, we are proving the following statement by
+induction on trees:
+forall t: Tree (is_bst(t) ==> forall j: int (is_in(j, t) == lookup(j, t)).
+
+Base case: t = empty. In that case lookup(j, t) and is_in (j, t)
+both yield false for any j: int.
+
+Inductive Hypothesis: For given binary search trees l and r,
+the functions lookup and is_in agree for all j: int.
+
+Inductive step: We show that for all i: int, the functions lookup
+and is_in agree on Node(l, i, r) if the latter is a binary search
+tree.
+
+So assume that Node(l, i, r) is a binary search tree, and let j
+be given.
+
+    Case 1: i == j. Then both functions return ’true’.
+
+    Case 2: j < i. As t is a binary search tree, we have that all
+    elements of the right subtree are greater than i, hence is_in(j,
+    r) will return false, so that is_in(j, t) will evalulate to
+    is_in(j, l). On the other hand, the function lookup will evaluate
+    to (i == j) || (j<i && lookup(j,l)) || (j>i && lookup(j,r).
+    Given that we have assumed that j < i, this evaluates to
+    lookup(i, l).
+
+As Node (l, i, r) is a binary search tree, we have by definition
+that both l and r are binary search trees, as well and we may
+conclude by the inductive hypothesis that lookup(i, l) and
+is_in(i, j) evaluate to the same value, as required.
+
+Case 2: i < j: this is analogous to the case above, with the
+roles of left / right subtree interchanged.
+*/
+
 
 
 // Exercise 2 Insertion – Elements
@@ -126,3 +154,115 @@ ensures is_bst (insert (j, t))
 // every element i of a tree t are elements of insert(j, t), and that every element of 
 // insert (j, t) is of this form. Dafny should prove these lemmas automatically. As in 
 // the previous Exercise, also give the proof of insert is in by hand in a comment.
+
+function insert (j: int, t: Tree): Tree {
+match t {
+    case Emp => Node (Emp, j, Emp)
+    case Node (l, i, r) =>
+        if (j < i) then Node (insert (j, l), i, r)
+        else if (j > i) then Node (l, i, insert (j, r))
+        else t
+    }
+}
+
+// ===============================
+// ======== MA BEGINS ============
+// ================================
+
+// Exercise 4, Minium Finding:
+
+// Due to the structure of a binary search tree, the smallest element will be stored at 
+// the leftmost position. This means we can compute the minimum of a non-empty binary 
+// search tree as follows:
+
+function min (t: Tree): int
+requires t != Emp {
+    match t { 
+        case Node (Emp, root, right) => root
+        case Node (left, root, right) => min(left)
+    }
+}
+
+function root_elt (t: Tree): int
+    requires t != Emp {
+    match t {
+        case Node (left, root, right) => root
+    }
+}
+
+// (a) Formulate a lemma min_in that asserts that the minimum (computed by the function min) of a 
+// non-empty tree is always an element of the tree. Dafny should prove this automatically. In a 
+// comment, give a proof of the statement by hand, stating clearly what you prove, the inductive 
+// hypothesis, the base case and the step case
+
+lemma min_in(t: Tree)
+requires is_binary_search_tree(t)
+requires t != Emp
+ensures is_in(min(t), t){
+
+} 
+
+/*
+Proof for the following:
+forall t: Tree (is_binary_search_tree(t) && t != Emp => is_in(min(t), t))
+
+Base Case:
+t = node(Emp, root, right)
+from the min function, 'case Node (Emp, root, right) => root'
+therefore we have t = root, and root is an element of t,
+thus min(t) is in t.
+
+Inductive Hypothesis
+min(l) is in l
+
+step case:
+tree = node(left, root, right), left is non-emty
+by definition min(t) = min(root) as left is Emp
+and a bst is sorted left to right.
+from the inductive hypothesis, min(left) is in left.
+Every element of left is also an element of the whole tree.
+therefore min(t) is in t in all cases.
+*/
+
+// (b) Give a proof, in Dafny, of the lemma min_left that asserts that the minimum of a binary search
+// tree (as computed by the function min) is always below the root node. Lemma min_in might be helpful.
+
+lemma min_left(t: Tree)
+requires t != Emp
+requires is_binary_search_tree(t)
+ensures min(t) <= root_elt(t){
+    match t
+    // Base Case where min(t) = main_node.
+    // means that min(t) <= root_element(t)
+        case Node(Emp, main_node, right) => 
+            assert min(t) == main_node;
+            assert root_elt(t) == main_node;
+        // Inductive Case
+        case Node(left, main_node, right) => 
+            min_in(left);
+            assert is_in(min(left), left);
+}
+
+// (c) Give a proof, in Dafny, of the lemma min_least that asserts the correctness of the function min. 
+// The lemma min_left might be helpful.
+lemma{:induction false} min_least(t: Tree)
+  requires t != Emp
+  requires is_binary_search_tree(t)
+  ensures forall x:int :: is_in(x, t) ==> min(t) <= x
+//Got stuck here, so had to go with a simple solution.
+{
+  match t
+    // Base case where left subtree is empty.
+    case Node(Emp, main_node, right_node) =>
+    assert min(t) == main_node;
+    assert root_elt(t) == main_node;
+    assert forall x:int :: is_in(x, t) ==> min(t) <= x;
+    // min(t) == main_node, so we just need to show main_node <= x.
+    // Step case for a left subtree that's not empty.
+    case Node(left_node, main_node, right_node) =>
+      min_least(left_node);
+      min_left(t);
+      assert min(t) <= main_node;
+      assert min(t) == min(left_node);
+      assert forall x:int :: is_in(x, t) ==> min(t) <= x;
+}
